refine_uniq removal

EventSystems/Refinement/Functional/Basic.lean
@@ -4,56 +4,32 @@ import EventSystems.Refinement.Relational.Basic
 
 class FRefinement {ACTX : outParam (Type u₁)} (AM)
                   {CTX : outParam (Type u₂)} (M)
-                  [Machine ACTX AM] [Machine CTX M] extends Refinement AM M where
+                  [Machine ACTX AM] [Machine CTX M] where
 
   lift (m : M): AM
 
-  lift_ref (m : M):
+  lift_safe (m : M):
     Machine.invariant m
-    → refine (lift m) m
-
-  refine_uniq (am am' : AM) (m : M):
-    Machine.invariant m
-    → refine am m → refine am' m
-    → am = am'
+    → Machine.invariant (lift m)
 
 open Refinement
 open FRefinement
 
-theorem lift_safe [Machine ACTX AM] [Machine CTX M] [instR:FRefinement AM M] (m : M):
+instance [Machine ACTX AM] [Machine CTX M] [FRefinement AM M]: Refinement AM M where
+  refine (am : AM) (m : M) := am = lift m
+
+  refine_safe (am : AM) (m : M) := by
+    simp
+    intros Hinv Ham
+    rw [Ham]
+    exact lift_safe m Hinv
+
+
+theorem lift_ref [Machine ACTX AM] [Machine CTX M] [instFR:FRefinement AM M] (m : M) :
   Machine.invariant m
-  → Machine.invariant (M:=AM) (lift m) :=
+  → refine (AM:=AM) (self:=instRefinementOfFRefinement) (lift m) m :=
 by
-  intro Hinv₁
-  have Href := FRefinement.lift_ref (self:=instR) m Hinv₁
-  apply refine_safe (M:=M) (lift m) m Hinv₁ Href
-
-@[simp]
-def defaultRefine {AM} [Machine ACTX AM] {M} [Machine CTX M]
-  (abs : M → AM) (am : AM) (m : M) :=
-  am = abs m
-
-theorem defaultRefine_safe {AM} [Machine ACTX AM] {M} [Machine CTX M]
-  (abs : M → AM)  (am : AM) (m : M) (Habs: Machine.invariant m → Machine.invariant (abs m)):
-    Machine.invariant m
-    → defaultRefine abs am m
-    → Machine.invariant am :=
-by
-  intros Hinv Href
-  unfold defaultRefine at Href
-  rw [Href]
-  apply Habs
-  assumption
-
-theorem defaultRefine_ref {AM} [Machine ACTX AM] {M} [Machine CTX M]
-  (abs : M → AM) (m : M) (am am' : AM):
-  Machine.invariant m
-    → defaultRefine abs am m → defaultRefine abs am' m
-    → am = am' :=
-by
-  simp
-  intros _ Href₁ Href₂
-  simp [*]
+  simp [refine]
 
 structure FREventSpec (AM) [Machine ACTX AM] (M) [Machine CTX M] [instfr: FRefinement AM M]
   {α β α' β'} (abstract : OrdinaryEvent AM α' β')
@@ -88,24 +64,18 @@ def FREventSpec.toREventSpec [Machine ACTX AM] [Machine CTX M] [instFR: FRefinem
     strengthening := fun m x => by
       intros Hinv Hgrd am Href
       have Hst := ev.strengthening m x Hinv Hgrd
-      have Href' := lift_ref (self:=instFR) m Hinv
-      have Huniq := refine_uniq (self:=instFR) am (lift m) m Hinv Href Href'
-      rw [Huniq]
-      exact Hst
+      simp [refine] at Href
+      rw [Href]
+      assumption
 
     simulation := fun m x => by
       simp
       intros Hinv Hgrd am Href
       have Hsim := ev.simulation m x Hinv Hgrd
       simp at Hsim
-      obtain ⟨Hsim₁, Hsim₂⟩ := Hsim
-      have Href' := lift_ref (self:=instFR) m Hinv
-      have Huniq := refine_uniq (self:=instFR) am (lift m) m Hinv Href Href'
-      rw [Huniq]
-      simp [Hsim₁]
-      rw [Hsim₂]
-      apply lift_ref
-      · apply ev.safety m x Hinv Hgrd
+      simp [refine] at Href
+      rw [Href]
+      exact Hsim
   }
 
 @[simp]
@@ -207,7 +177,8 @@ structure InitFREventSpec (AM) [Machine ACTX AM] (M) [Machine CTX M] [instFR: FR
 @[simp]
 def InitFREventSpec.toInitREventSpec [Machine ACTX AM] [Machine CTX M] [instFR: FRefinement AM M]
   {abs : InitEvent AM α' β'}
-  (ev : InitFREventSpec (instFR:=instFR) (α:=α) (β:=β) (α':=α') (β':=β') abs) : InitREventSpec (instR:=instFR.toRefinement) (α:=α) (β:=β) (α':=α') (β':=β') abs :=
+  (ev : InitFREventSpec (instFR:=instFR) (α:=α) (β:=β) (α':=α') (β':=β') abs)
+    : InitREventSpec (AM:=AM) (M:=M) (α:=α) (β:=β) (α':=α') (β':=β') abs :=
   {
     toInitEventSpec := ev.toInitEventSpec
     lift_in := ev.lift_in
